\documentclass{beamer}

\usepackage{amssymb}
\usepackage{amsfonts}
\usepackage{amsmath}
\usepackage{amsthm}
\usepackage{setspace}
\usepackage{longtable}
\usepackage{graphicx}
\usepackage{mathtools}
\usepackage{color}
\usepackage{array}
\usepackage{calc} 
\usepackage{bm}
\usepackage{caption}
\usepackage{float}

\usetheme{CambridgeUS}
\useoutertheme{infolines}
%numbering
\setbeamercolor{background canvas}{bg=white}
\setbeamersize{text margin left=1cm,text margin right=1cm}

\title[AI1110  Assignment-8]{ASSIGNMENT-8}
\subtitle{AI1110}
\author[]{MUKUNDA REDDY \\ AI21BTECH11021}
\date

\begin{document}
  \begin{frame}
      \titlepage
  \end{frame}
  
  \begin{frame}{Outline}
      \tableofcontents
  \end{frame}
  
  \section{Question}
  \begin{frame}{Exercise 7-13}
       The random variables $X_i$ are i.i.d.
       with moment function $ \phi_x (s) = 
       E\{e^{sx_i}\} \forall i $.The random variable n takes the values 0,1,2... and its 
       moment function equals $\Gamma_n \{z\} = E\{z^n\}$.Show that if
       $$ y = \sum^{n}_{i=1} x_i,\: \text{then  }  \phi_y (s) = 
       E\{e^{sy}\} = \Gamma_n \{\phi_x (s)\}  $$
  \end{frame}
  
  \section{Solution}
  \begin{frame}{Solution}
     Given $y = x_1+x_2+...+x_n$ and given $ \phi_x (s) = 
       E\{e^{sx_i}\} \forall i $  also by the
       independence of the random variable $x_i$ we have
       we have 
      \begin{align}
      E\{e^{sy}|n=k\} &= E\{e^{s(x_1+x_2..x_k)}\} \nonumber \\
     &= E\{e^{sx_1}\}...E\{e^{sx_k}\} \nonumber \\
     &= \phi_x (s)...\phi_x (s) \text{(k times)} \nonumber \\
        \label{eq1} &= \phi_x ^{k} (s) 
      \end{align}
  \end{frame}
  
  \begin{frame}{Solution}
      \begin{align}
        \phi_y \{s\} &= E\{e^{sy}\} \nonumber  \\
           &=   E\{E\{e^{sy}\}\} \text{ Since E\{E\{X\}\} = E\{X\} } \nonumber \\
           &=  E\{ \phi_x ^{n} (s)\} \text{ from } \eqref{eq1} 
      \end{align}
      We know that $E\{z^{n}\} = \Gamma_n (z)$.
      let's Consider $z=\phi_x (s)$ then we have
      \begin{equation}
      \phi_y \{s\} &= E\{e^{sy}\}  = \Gamma_n [\phi_x (s) ]    
      \end{equation}
  \end{frame}
\end{document}